MECMAR/Notation.v
@@ -1,15 +1,23 @@
-From Coq Require Import List.
-From Warblre Require Import Result Base Patterns.
+From Coq Require Import ZArith List.
+From Warblre Require Import Result Base.
 
 (** 22.2.2.1 Notation *)
 Module Notation.
+  (*  A CharSet is a mathematical set of characters. In the context of a Unicode pattern, “all characters” means
+      the CharSet containing all code point values; otherwise “all characters” means the CharSet containing all
+      code unit values. *)
+  Definition CharSet := Character -> bool.
 
+  (*  A CaptureRange is an ordered pair (startIndex, endIndex) that represents the range of characters included
+      in a capture, where startIndex is an integer representing the start index (inclusive) of the range within
+      Input, and endIndex is an integer representing the end index (exclusive) of the range within Input. For any
+      CaptureRange, these indices must satisfy the invariant that startIndex ≤ endIndex. *)
   Module CaptureRange.
     Record type := make {
-      startIndex: non_neg_integer; (* inclusive *)
-      endIndex: non_neg_integer; (* exclusive *)
+      startIndex: integer; (* inclusive *)
+      endIndex: integer; (* exclusive *)
 
-(*           invariant: startIndex <= endIndex; *)
+      (* invariant: startIndex <= endIndex; *)
     }.
 
     Module Exports.
@@ -19,14 +27,20 @@ Module Notation.
   End CaptureRange.
   Export CaptureRange.Exports.
 
+  (*  A MatchState is an ordered triple (input, endIndex, captures) where input is a List of characters
+      representing the String being matched, endIndex is an integer, and captures is a List of values, one for
+      each left-capturing parenthesis in the pattern. States are used to represent partial match states in the
+      regular expression matching algorithms. The endIndex is one plus the index of the last input character
+      matched so far by the pattern, while captures holds the results of capturing parentheses. The nth element
+      of captures is either a CaptureRange representing the range of characters captured by the nth set of
+      capturing parentheses, or undefined if the nth set of capturing parentheses hasn't been reached yet. Due
+      to backtracking, many States may be in use at any time during the matching process. *)
   Module MatchState.
     Record type := make {
       input: list Character;
-      endIndex: non_neg_integer; (* one plus the index of the last input character matched so far *)
+      endIndex: integer; (* one plus the index of the last input character matched so far *)
       captures: DMap.t CaptureRange;
     }.
-
-(*         Definition remainingCharsCount (x: type) := (length (input x)) - (endIndex x). *)
 
     Module Exports.
       Notation MatchState := type.
@@ -35,37 +49,37 @@ Module Notation.
   End MatchState.
   Export MatchState.Exports.
 
-  (* «  The nth element of captures is either a CaptureRange representing 
-        the range of characters captured by the nth set of capturing parentheses, 
-        or undefined if the nth set of capturing parentheses hasn't been reached 
-        yet. » 
-        This sounds imprecise: the capture group may have been reached, but reset
-  *)
-
-  Notation "ls '[' i ']'" := (match nth_error ls i with
-  | Some x => Success x
-  | None => assertion_failed
-  end) (at level 98, left associativity).
-
-  Inductive Failures :=
-  | Mismatch
-  | OutOfFuel
-  | AssertionFailed.
-
-  Definition MatchResult := Result MatchState Failures.
+  (* A MatchResult is either a MatchState or the special token failure that indicates that the match failed. *)
+  Definition MatchResult := Result MatchState MatchFailure.
   #[export]
-  Instance assertion_error: AssertionError Failures := { f := AssertionFailed }.
+  Instance assertion_error: Result.AssertionError MatchFailure := { f := AssertionFailed }.
   Notation failure := (Failure Mismatch).
   Notation out_of_fuel := (Failure OutOfFuel).
+  Notation assertion_failed := (Failure AssertionFailed).
 
+  (*  A MatcherContinuation is an Abstract Closure that takes one MatchState argument and returns a
+      MatchResult result. The MatcherContinuation attempts to match the remaining portion (specified by the
+      closure's captured values) of the pattern against Input, starting at the intermediate state given by its
+      MatchState argument. If the match succeeds, the MatcherContinuation returns the final MatchState that it
+      reached; if the match fails, the MatcherContinuation returns failure. *)
   Definition MatcherContinuation := MatchState -> MatchResult.
 
+  (*  A Matcher is an Abstract Closure that takes two arguments—a MatchState and a MatcherContinuation—
+      and returns a MatchResult result. A Matcher attempts to match a middle subpattern (specified by the
+      closure's captured values) of the pattern against the MatchState's input, starting at the intermediate state
+      given by its MatchState argument. The MatcherContinuation argument should be a closure that matches
+      the rest of the pattern. After matching the subpattern of a pattern to obtain a new MatchState, the Matcher
+      then calls MatcherContinuation on that new MatchState to test if the rest of the pattern can match as well.
+      If it can, the Matcher returns the MatchState returned by MatcherContinuation; if not, the Matcher may try
+      different choices at its choice points, repeatedly calling MatcherContinuation until it either succeeds or all
+      possibilities have been exhausted. *)
   Definition Matcher := MatchState -> MatcherContinuation -> MatchResult.
 
   (** 22.2.2.1.1 RegExp Records *)
   Record RegExp := {
   }.
 
+  (** Additional datatypes which are never properly defined. *)
   Inductive direction :=
   | forward
   | backward
@@ -79,3 +93,4 @@ Module Notation.
     end.
   End Direction.
 End Notation.
+Export Notation.
